proofs/x86-64/avx2/ml_dsa_65/keygen.ec
@@ -1,4 +1,4 @@
-require import AllCore List (* IntDiv RealExp StdBigop *).
+require import AllCore List IntDiv  RealExp (* StdBigop *).
 
 from Jasmin require import JModel_x86.
 
@@ -13,20 +13,82 @@ import CDR Round Zq PolyReduceZq BigZMod.
 
 (* require import ArrayExtra JWord_extra EclibExtra JWordList. *)
 
-require import Array32 Array64 Array128 Array256 Array320 Array640 Array768 Array1280 Array1536 Array1920 Array1952 Array2496 Array4032 Array7680.
+require import Array32 Array64 Array128 Array256 Array320 Array416 Array640 Array768 Array1280 Array1536 Array1920 Array1952 Array2496 Array4032 Array7680.
 require import WArray32 WArray1952 WArray4032.
 
 require import Bindings.
+require import BitEncoding.
+import BitChunking.
+
+lemma size_BitsToBytes l :  size (BitsToBytes l) = (size l) %/ 8.
+rewrite /BitsToBytes size_map size_chunk //. 
+qed.
+
+lemma size_SimpleBitPack _p b : 1 <= b => size (SimpleBitPack _p b) = (ilog 2 b + 1) * n %/ 8.
+move => Hb.
+rewrite /SimpleBitPack /=  size_BitsToBytes (size_flatten_ctt (ilog 2 b + 1)).
++ move => l; rewrite mapP => He; elim He => c /= [# ?->].
+  rewrite /IntegerToBits BS2Int.size_int2bs;smt(ilog_ge0).
+by rewrite size_map size_to_list.
+qed.
+
+lemma size_kflatten_SimpleBitPack (v : W32.t Array1536.t) b:
+   1 <= b =>
+    size (flatten (map (fun (p : poly) => SimpleBitPack p b) (to_list (liftu_wpolykvec (kvec_unflatten256 v))))) = kvec * (ilog 2 b + 1) * n %/ 8.
+move => Hb.
+rewrite (size_flatten_ctt ((ilog 2 b + 1) * n %/ 8)).
++ move => l; rewrite mapP => He;  elim He => p /= [# ? ->].
+  rewrite size_SimpleBitPack /= /#.
+by rewrite size_map size_to_list mldsa65_kvec /= /#.
+qed.
+
+lemma size_BitPack _p b1 b2 : 1 <= (b1 + b2) => size (BitPack _p b1 b2) = (ilog 2 (b1 + b2) + 1) * n %/ 8.
+move => Hb.
+rewrite /BitPack /=  size_BitsToBytes (size_flatten_ctt (ilog 2 (b1 + b2) + 1)).
++ move => l; rewrite mapP => He; elim He => c /= [# ?->].
+  rewrite /IntegerToBits BS2Int.size_int2bs. smt(ilog_ge0).
+by rewrite size_map size_to_list.
+qed.
+
+lemma size_lflatten_BitPack (v : W32.t Array1280.t) b1 b2:
+  1 <= (b1 + b2) =>
+   size (flatten (map (fun (p : poly) => BitPack p b1 b2) (to_list (lifts_wpolylvec (lvec_unflatten256 v))))) = lvec *  (ilog 2 (b1 + b2) + 1) * n %/ 8.
+move => Hb.
+rewrite (size_flatten_ctt ((ilog 2 (b1 + b2) + 1) * n %/ 8)).
++ move => l; rewrite mapP => He;  elim He => p /= [# ? ->].
+  rewrite size_BitPack /= /#.
+by rewrite size_map size_to_list mldsa65_lvec /= /#.
+qed.
+
+lemma size_kflatten_BitPack (v : W32.t Array1536.t) b1 b2:
+  1 <= (b1+b2) =>
+   size (flatten (map (fun (p : poly) => BitPack p b1 b2) (to_list (lifts_wpolykvec (kvec_unflatten256 v))))) = kvec *  (ilog 2 (b1 + b2) + 1) * n %/ 8.
+move => Hb.
+rewrite (size_flatten_ctt ((ilog 2 (b1 + b2) + 1) * n %/ 8)).
++ move => l; rewrite mapP => He;  elim He => p /= [# ? ->].
+  rewrite size_BitPack /= /#.
+by rewrite size_map size_to_list mldsa65_kvec /= /#.
+qed.
+
+lemma get256_init_32_8 (a : W8.t Array32.t) k:
+   0 <= k < 32 =>
+    (get256_direct (WArray32.init8 ("_.[_]" a)) 0 \bits8 k) = a.[k].
+move => kb.
+rewrite WArray32.get256E pack32E wordP => i ib.
+rewrite /(\bits8) initiE 1:/# /= initiE 1:/# /= initiE 1:/# /= initiE 1:/# /#.
+qed.
 
 lemma keygen_internal
     (RO <: LeakyRO):
     equiv [ MLDSA(MLDSA_XOFA, MLDSA_XOFS, RO).keygen_derand ~ M.__keygen_internal :
-       Bytes32.to_list arg{1} = to_list arg{2}.`3
+       arg{1} = Bytes32.of_list (to_list arg{2}.`3)
      ==>
-       BytesPK.to_list res{1}.`2 = to_list res{2}.`1 /\
-       BytesSK.to_list res{1}.`1 = to_list res{2}.`2
+       res{1}.`2 = BytesPK.of_list (to_list res{2}.`1) /\
+       res{1}.`1 = BytesSK.of_list (to_list res{2}.`2)
    ].
 proof.
+have Eta_val := mldsa65_Eta.
+have Hlvec := mldsa65_lvec.
 have Hkvec := mldsa65_kvec.
 proc => /=.
 seq 0 13 : #pre; 1: by auto.
@@ -34,34 +96,27 @@ seq 0 13 : #pre; 1: by auto.
 (* expanding seeds *)
 sp 2 0.
 seq 0 2 : (#pre /\
- to_list prf_output{2} =
-   Bytes32.to_list rho{1} ++ Bytes64.to_list rhop{1} ++ Bytes32.to_list _K{1}).
+ prf_output{2} =
+   Array128.of_list witness (Bytes32.to_list rho{1} ++ Bytes64.to_list rhop{1} ++ Bytes32.to_list _K{1})).
 + admit. (* TODO: REFACTORING TO USE FORMOSA-KECCAK *)
 
 (* expanding A *)
-seq 1 2: (#pre /\ liftu_wpolymat (mat_unflatten256 matrix_A{2}) = _A{1} /\
+sp;seq 1 1: (#pre /\ liftu_wpolymat (mat_unflatten256 matrix_A{2}) = _A{1} /\
             wpolymat_urng (mat_unflatten256 matrix_A{2}) 1).
 + ecall{1} (ExpandA_correct rho{1}).
   ecall{2} (matrix_A_correct seed_for_matrix_A{2}).
-  auto => /> &1 &2 _ _ H.
-  have Hn : forall i, 0 <= i < 128 => prf_output{2}.[i] =
-                     nth witness (Bytes32.to_list rho{1} ++ Bytes64.to_list rhop{1} ++ Bytes32.to_list _K{1}) i.
-  + by  move => kk kkb;rewrite -H  ?size_to_list 1:/#  !get_to_list.
-  move => rr -> ?;congr.
-  apply Bytes32.tP => k kb;rewrite Bytes32.get_of_list // get_to_list initiE 1:/# /=.  
-  by rewrite  Hn 1:/# -catA nth_cat ?Bytes32.size_to_list ifT 1:/#  Bytes32.get_to_list.
+  auto => /> &1 &2 ? rr ->?.
+  + congr; apply Bytes32.tP => k kb.
+    rewrite Bytes32.get_of_list 1:/# get_to_list initiE 1:/# get_of_list 1:/# nth_cat ifT.
+    + by rewrite size_cat;smt(Bytes32.size_to_list).
+    by rewrite nth_cat ifT;smt(Bytes32.size_to_list).
 
 (* expanding noise *)
 seq 0 2 : (#pre
-     /\ to_list seed_for_error_vectors{2} = Bytes64.to_list rhop{1}
-     /\ to_list seed_for_signing{2} = Bytes32.to_list _K{1}).
-+ auto => /> &1 &2 _ _ H ?.
-  have Hn : forall i, 0 <= i < 128 => prf_output{2}.[i] =
-                     nth witness (Bytes32.to_list rho{1} ++ Bytes64.to_list rhop{1} ++ Bytes32.to_list _K{1}) i.
-  + by  move => kk kkb;rewrite -H  ?size_to_list 1:/#  !get_to_list.
-  split;apply (eq_from_nth witness);rewrite size_to_list ?Bytes32.size_to_list ?Bytes64.size_to_list //= => k kb; rewrite initiE 1:/# /= Hn 1:/# -catA nth_cat ?Bytes32.size_to_list ifF 1:/# nth_cat ?Bytes64.size_to_list.
-  + by rewrite ifT 1:/# Bytes64.get_to_list /#.
-  by rewrite ifF 1:/# Bytes32.get_to_list /#.
+     /\ seed_for_error_vectors{2} = Array64.of_list witness (Bytes64.to_list rhop{1})
+     /\ seed_for_signing{2} = Array32.of_list witness (Bytes32.to_list _K{1})).
++ auto => /> &1 &2 ??.
+  by split; rewrite tP => k kb; rewrite initiE 1:/# /= get_of_list 1:/# get_of_list 1:/# !nth_cat ?size_cat ?Bytes32.size_to_list ?Bytes64.size_to_list /#.
 
 seq 1 1 : (#pre
      /\ lifts_wpolylvec (lvec_unflatten256 s1{2}) = s1{1}
@@ -70,8 +125,7 @@ seq 1 1 : (#pre
      /\ wpolykvec_srng (kvec_unflatten256 s2{2}) Eta Eta).
 + ecall{1} (ExpandS_correct rhop{1}).
   ecall{2} (error_vectors_correct seed_for_error_vectors{2}).
-  auto => /> &1 &2 _ _ _ _ ->.
-  by rewrite !Bytes64.to_listK => _ rr -> ? -> ?.
+  by auto => /> &1 &2 ?? rr -> ?->?; split;congr;congr;rewrite Bytes64.tP => k kb;rewrite Bytes64.get_of_list 1:/# get_to_list get_of_list /#.
 
 proc change {2} [10..11] : [s1p : W32.t Array1280.t] {
    s1p <@ M.row_vector__ntt(s1);
@@ -96,19 +150,73 @@ seq 2 7 : (#pre
   wp; ecall {1} (skEncode_corr rho{1} _K{1} tr{1} s1{1} s2{1} t0{1}).
   wp; ecall {1} (pkEncode_corr rho{1} t1{1}).
 
-  auto => /> &1 &2 ?????????? rr1 Hrr11 rr2 Hrr21 Hrr22 rr3 Hrr31  rr4 Hrr41 Hrr42 rr5 Hrr5.
-  split.
-  + rewrite BytesPK.of_listK. 
-    + rewrite size_cat Bytes32.size_to_list (size_flatten_ctt 320).
-      + move =>x; rewrite mapP => He; elim He => xx /=.
-        rewrite /to_list mkseqP => [# He ->]; elim He => xxx /= => [# ??].
-        rewrite mapiE 1:/# initiE 1:/# /= => ->.
-        rewrite SimpleBitPack_liftE. admit.
-        by rewrite size_to_list.
-      by rewrite size_map /= size_to_list /#.
-    admit.
-  admit.
-
-admit.
-
+  auto => /> &1 &2 ?????? rr1 Hrr1 rr2 Hrr2 rr3 Hrr3  rr4 Hrr4.
+  split;congr.
+  + apply (eq_from_nth witness); 1: by rewrite size_cat Bytes32.size_to_list size_kflatten_SimpleBitPack 1:/# size_to_list /#.
+    move => k;rewrite size_cat Bytes32.size_to_list size_kflatten_SimpleBitPack 1:/# /= => Hk.
+    rewrite initiE 1:/# /= nth_cat Bytes32.size_to_list; case (k < 32) => ?.
+    + rewrite ifF 1:/# initiE 1:/# /= ifT 1:/# get256_init_32_8 1:/# initiE 1:/# get_of_list 1:/# nth_cat ifT.
+      + by rewrite size_cat Bytes32.size_to_list Bytes64.size_to_list /#.
+      by rewrite nth_cat Bytes32.size_to_list /#.
+    rewrite ifT 1:/# (nth_flatten witness 320).
+    + rewrite allP => x; rewrite mapP => He; elim He => p /= [# ? ->].
+      by rewrite size_SimpleBitPack /#.
+      rewrite (nth_map witness) /=; 1: by rewrite size_to_list /#.
+    move : Hrr3; rewrite kvec_unflatten320iE 1:/# => ->.
+    rewrite mapiE 1:/# /= mapiE 1:/# /= get_of_list 1:/#.
+    congr;congr; last by auto.
+    by rewrite mapiE 1:/#.
+  + apply (eq_from_nth witness).
+    + rewrite !size_cat !Bytes32.size_to_list Bytes64.size_to_list.
+      by rewrite size_to_list size_lflatten_BitPack 1:/# !size_kflatten_BitPack 1,2:/# Eta_val Hlvec /= Hkvec /=.
+    move => i; rewrite !size_cat !Bytes32.size_to_list Bytes64.size_to_list size_lflatten_BitPack 1:/# !size_kflatten_BitPack 1,2:/# Eta_val Hlvec /= Hkvec /= => Hi.
+    rewrite !nth_cat.
+    rewrite !size_cat !Bytes32.size_to_list Bytes64.size_to_list size_lflatten_BitPack 1:/# !size_kflatten_BitPack 1:/# Hlvec /= Hkvec /=.
+    rewrite initiE 1:/# /= initiE 1:/# /= initiE 1:/# /= initiE 1:/# /= initiE 1:/# /=.
+    case (i < 1536) => ?; last first.
+    + rewrite ifT 1:/#.
+      move : Hrr4; rewrite kvec_unflatten416iE 1:/# => ->.
+      rewrite mapiE 1:/# /= get_of_list 1:/# (nth_flatten witness 416).
+      + rewrite allP => x; rewrite mapP => He; elim He => p /= [# ? ->].
+        by rewrite size_BitPack /#.
+      by rewrite (nth_map witness) /=; rewrite ?size_to_list /#.
+    case (i < 768) => ?; last first.
+    + rewrite ifF 1:/# ifF 1:/# ifT 1:/#.
+      move : Hrr2; rewrite kvec_unflatten128iE 1:/# => ->.
+      rewrite mapiE 1:/# /= get_of_list 1:/# (nth_flatten witness 128).
+      + rewrite allP => x; rewrite mapP => He; elim He => p /= [# ? ->].
+        by rewrite size_BitPack /#.
+      by rewrite (nth_map witness) /=; rewrite ?size_to_list /#.
+    case (i < 128) => ?; last first.
+    + rewrite ifF 1:/# ifF 1:/# ifF 1:/# ifT 1:/#.
+      move : Hrr1; rewrite lvec_unflatten128iE 1:/# => ->.
+      rewrite mapiE 1:/# /= get_of_list 1:/# (nth_flatten witness 128).
+      + rewrite allP => x; rewrite mapP => He; elim He => p /= [# ? ->].
+        by rewrite size_BitPack /#.
+      by rewrite (nth_map witness) /=; rewrite ?size_to_list /#.
+    case (i < 64) => ?; last first.
+    + rewrite ifF 1:/# ifT 1:/# get_of_list 1:/# Bytes64.get_to_list;congr;congr;congr.
+      apply (eq_from_nth witness).
+      + rewrite !size_cat !Bytes32.size_to_list.
+        by rewrite size_to_list size_kflatten_SimpleBitPack /#.
+      move => k; rewrite !size_cat !Bytes32.size_to_list size_kflatten_SimpleBitPack //= => ?.
+      rewrite initiE 1:/# /= initiE 1:/# /=.
+      case (k < 32) => ?.
+      + rewrite ifF 1:/# ifT 1:/# nth_cat ifT 1:/# Bytes32.get_to_list get256_init_32_8 1:/# initiE 1:/# get_of_list 1:/#.
+        by rewrite nth_cat size_cat Bytes32.size_to_list ifT 1:/# nth_cat Bytes32.size_to_list ifT 1:/# Bytes32.get_to_list /#.
+      rewrite ifT 1:/# nth_cat ifF; 1: by rewrite Bytes32.size_to_list  /=.
+      move : Hrr3;rewrite kvec_unflatten320iE 1:/# => ->.
+      rewrite mapiE 1:/# /= get_of_list 1:/# (nth_flatten witness 320).
+      + rewrite allP => x; rewrite mapP => He; elim He => p /= [# ? ->].
+        by rewrite size_SimpleBitPack /#.
+      by rewrite (nth_map witness) /=; rewrite ?size_to_list /#.
+    case (i < 32) => ?.
+    + rewrite ifF 1:/# ifF 1:/# ifF 1:/# ifF 1:/# ifF 1:/#. 
+      rewrite /get8 initiE 1:/# initiE 1:/# /= set256E initiE 1:/# /= ifT 1:/# get256_init_32_8 1:/# initiE 1:/# get_of_list 1:/#.
+      rewrite  nth_cat ifT; 1: by rewrite size_cat Bytes32.size_to_list  /#.
+      rewrite nth_cat ifT;1:by rewrite  Bytes32.size_to_list  /#.
+      by rewrite Bytes32.get_to_list /#.
+    by rewrite ifF 1:/# ifF 1:/# ifF 1:/# ifF 1:/# ifT 1:/# get256_init_32_8 1:/# initiE 1:/# /=.
+    
+admit. (* Algebra *)
 qed.
